Add complex test

Source/IntegrationTests/TestFiles/LitTests/LitTest/comp/placeholders/complex/randomCSharp.dfy
@@ -1,13 +1,35 @@
 
-module RandomCSharp replaces Random {
+module RandomCSharp replaces DfyRandom {
+  import CSharpSystem
+  import Interop
+  
   method GetRandomNat ... {
-    var random := new Random();
-    return 0;
+    // Ignore the ceiling parameter for now
+    var random := new CSharpSystem.Random();
+    var resultInt32 := random.Next();
+    var resultInt := Interop.Int32ToInt(resultInt32);
+    return resultInt as nat;
   }
 }
 
+module Interop {
+  import CSharpSystemTypes
+  
+  function {:extern} Int32ToInt(value: CSharpSystemTypes.Int32): int
+}
+
+module {:extern "System"} CSharpSystemTypes {
+  class {:extern "Int32" } Int32 { }
+}
+
 module {:extern "System"} CSharpSystem {
+  import Interop
+  import opened CSharpSystemTypes
+  
   class {:extern "Random" } Random {
-    constructor() { }
+    constructor {:extern} () { }
+    
+    method {:extern} Next() returns (r: Int32)
+      ensures Interop.Int32ToInt(r) >= 0
   }
 }
